

# Rotation

Rado Faletič

## 1 2-dimensions

Given a vector  $(x, y) = (r \cos \theta, r \sin \theta) \in \mathbb{R}^2$ , we can rotate this vector through an angle  $\theta'$  by applying the following matrix:

$$\begin{bmatrix} x' \\ y' \end{bmatrix} = \begin{bmatrix} \cos \theta' & -\sin \theta' \\ \sin \theta' & \cos \theta' \end{bmatrix} \begin{bmatrix} x \\ y \end{bmatrix}$$

PROOF:

$$\begin{aligned} x' &= r \cos(\theta + \theta') & y' &= r \sin(\theta + \theta') \\ &= r (\cos \theta \cos \theta' - \sin \theta \sin \theta') & &= r (\cos \theta \sin \theta' + \sin \theta \cos \theta') \\ &= r \cos \theta \cos \theta' - r \sin \theta \sin \theta' & &= r \cos \theta \sin \theta' + r \sin \theta \cos \theta' \\ &= x \cos \theta' - y \sin \theta' & &= x \sin \theta' + y \cos \theta' \end{aligned}$$

## 2 3-dimensions

Given a vector  $(x, y, z) = (r \sin \phi \cos \theta, r \sin \phi \sin \theta, r \cos \phi) \in \mathbb{R}^3$ , we can rotate this vector through angles  $\theta'$  and  $\phi'$  by applying the following non-linear transformation:

$$\begin{bmatrix} x' \\ y' \\ z' \end{bmatrix} = \begin{bmatrix} x \cos \phi' \cos \theta' - y \cos \phi' \sin \theta' + z \sin \phi' (\cos \theta \cos \theta' - \sin \theta \sin \theta') \\ x \cos \phi' \sin \theta' + y \cos \phi' \cos \theta' + z \sin \phi' (\cos \theta \sin \theta' + \sin \theta \cos \theta') \\ z \cos \phi' - r \sin \phi \sin \phi' \end{bmatrix}$$

PROOF:

$$\begin{aligned} x' &= r \sin (\phi + \phi') \cos (\theta + \theta') \\ &= r (\sin \phi \cos \phi' + \cos \phi \sin \phi') (\cos \theta \cos \theta' - \sin \theta \sin \theta') \\ &= r \sin \phi \cos \phi' \cos \theta \cos \theta' - r \sin \phi \cos \phi' \sin \theta \sin \theta' \\ &\quad + r \cos \phi \sin \phi' \cos \theta \cos \theta' - r \cos \phi \sin \phi' \sin \theta \sin \theta' \\ &= x \cos \phi' \cos \theta' - y \cos \phi' \sin \theta' + z \sin \phi' (\cos \theta \cos \theta' - \sin \theta \sin \theta') \\ y' &= r \sin (\phi + \phi') \sin (\theta + \theta') \\ &= r (\sin \phi \cos \phi' + \cos \phi \sin \phi') (\sin \theta \cos \theta' + \cos \theta \sin \theta') \\ &= r \sin \phi \cos \phi' \sin \theta \cos \theta' + r \sin \phi \cos \phi' \cos \theta \sin \theta' \\ &\quad + r \cos \phi \sin \phi' \sin \theta \cos \theta' + r \cos \phi \sin \phi' \cos \theta \sin \theta' \\ &= y \cos \phi' \cos \theta' + x \cos \theta' \sin \theta' + z \sin \theta' (\sin \theta \cos \theta' + \cos \theta \sin \theta') \\ &= x \cos \theta' \sin \theta' + y \cos \phi' \cos \theta' + z \sin \theta' (\cos \theta \sin \theta' + \sin \theta \cos \theta') \\ z' &= r \cos (\phi + \phi') \\ &= r \cos \phi \cos \phi' - r \sin \phi \sin \phi' \\ &= z \cos \phi' - r \sin \phi \sin \phi' \end{aligned}$$